PoS/Semantics.v
@@ -3,9 +3,58 @@ Require Import ssreflect ssrbool ssrnat eqtype ssrfun seq.
 From mathcomp
 Require Import path.
 Require Import Eqdep pred prelude idynamic ordtype pcm finmap unionmap heap coding. 
+Require Import Protocol.
 Set Implicit Arguments.
 Unset Strict Implicit.
 Unset Printing Implicit Defensive.
 
 
 (* Network semantics *)
+Section PacketEqType.
+
+Fixpoint eqpkt a b :=
+  ((src a) == (src b)) && ((dst a) == (dst b)) &&
+  match (msg a), (msg b) with
+  | NullMsg, NullMsg => true
+  | NullMsg, _ => false
+  | Addr idA prsA, Addr idB prsB => (idA == idB) && (prsA == prsB)
+  | Addr _ _, _ => false
+  | Connect idA, Connect idB => (idA == idB)
+  | Connect _, _ => false
+  end.
+
+Lemma eqpktP : Equality.axiom eqpkt.
+Proof.
+Admitted.
+
+Canonical Packet_eqMixin := EqMixin eqpktP.
+Canonical Packet_eqType := EqType Packet Packet_eqMixin.
+
+End PacketEqType.
+
+
+Definition PacketSoup := seq Packet.
+
+Definition StateMap := union_map [ordType of nid] State.
+
+Record World :=
+  mkW {
+    localState : StateMap;
+    inFlightMsgs : PacketSoup;
+  }.
+
+Print Equality.sort.
+
+Inductive reliable_step (w w' : World) : Prop :=
+| step_msg (p : Packet) (st' : State) (ms : ToSend) of
+      p \in (inFlightMsgs w) &
+      match (find (dst p) (localState w)) with
+      | Some(st) => updS st (msg p) = (st', ms)
+      | _ => false
+      end &
+
+      reliable_step w
+        (mkW
+           (upd (dst p) st' (localState w))
+           (ms ++ rem p (inFlightMsgs w))
+        ).
